theories/tree_test.v
@@ -5,9 +5,12 @@ From det Require Import finmap ctx lang tree tree_prop.
 Notation "X ||[ Y s ]" := (Or X s Y) (at level 3).
 Notation "` X" := ((ACall X)) (at level 3). *)
 
+Definition prop := b (d Pred).
+Definition build_arr m := arr m prop prop.
+
 Definition build_progr l := {|
-    modes := [fmap].[IKp 0 <- [::o]].[IKp 1 <- [::o]].[IKp 2 <- [::o]].[IKp 200 <-  [::]];
-    sig := empty_sig;
+    (* modes := [fmap].[IKp 0 <- [::o]].[IKp 1 <- [::o]].[IKp 2 <- [::o]].[IKp 200 <-  [::]]; *)
+    sig := [fmap].[IKp 0 <- build_arr o].[IKp 1 <- build_arr o].[IKp 2 <- build_arr o].[IKp 200 <- prop];
     rules := l;
 |}.
 
